Update gh-pages branch with current main (#632)
* Add Gemfiles and change font (#619)

* Wire up clock and reset in sequential blackboxes (#622)

* Rename peel/unpeel to packv and unpackv (#612)

* Rename multistep to simulate (#626)

* aes_cipher_core: Working check-in (#624)

* Remove unIdent (#627)

* Create test benches based on FIPS for subroutine netlists (#599)

* Renaming and tweaks to trees (#628)

* renaming and tweaks to trees

* expose Identity in haskell

* Rename/move files in Cava (#631)

* update tutorial after merge

Co-authored-by: Satnam Singh <satnam@google.com>
Co-authored-by: Ben Blaxill <benblaxill@google.com>

acorn-examples/xilinx/XilinxAdderTree.v
@@ -29,7 +29,7 @@ Require Import ExtLib.Structures.Monads.
 
 Require Import Cava.Cava.
 Require Import Cava.Acorn.Acorn.
-Require Import Cava.Acorn.XilinxAdder.
+Require Import Cava.Lib.XilinxAdder.
 Existing Instance CavaCombinationalNet.
 
 Section WithCava.
@@ -41,9 +41,9 @@ Section WithCava.
   (****************************************************************************)
   Definition adderTree {sz: nat}
              (n: nat)
-    : signal (Vec (Vec Bit sz) (2^(S n))) ->
+    : signal (Vec (Vec Bit sz) (2^n)) ->
       cava (signal (Vec Bit sz)) :=
-    peel >=> tree defaultSignal n xilinxAdder.
+    tree (fun '(x,y) => xilinxAdder x y).
 
   (****************************************************************************)
   (* An adder tree with 2 inputs.                                             *)
@@ -51,7 +51,7 @@ Section WithCava.
   Definition adderTree2 {sz: nat}
                         (v : signal (Vec (Vec Bit sz) 2))
                         : cava (signal (Vec Bit sz))
-    := adderTree 0 v.
+    := adderTree 1 v.
 
   (******************************************************************************)
   (* An adder tree with 4 inputs.                                               *)
@@ -59,7 +59,7 @@ Section WithCava.
   Definition adderTree4 {sz: nat}
                         (v : signal (Vec (Vec Bit sz) 4))
                         : cava (signal (Vec Bit sz))
-    := adderTree 1 v.
+    := adderTree 2 v.
 
 End WithCava.
 
@@ -76,16 +76,15 @@ Local Open Scope nat_scope.
 Local Open Scope vector_scope.
 
 Definition v0_v1 : Vector.t (Bvector 8) 2 := [v0; v1].
-Definition v0_plus_v1 : Bvector 8 := unIdent (adderTree2 v0_v1).
+Definition v0_plus_v1 : Bvector 8 := adderTree2 v0_v1.
 Example sum_vo_v1 : v0_plus_v1 = N2Bv_sized 8 21.
 Proof. reflexivity. Qed.
 
 Local Open Scope N_scope.
 
 Definition v0_v1_v2_v3 := [v0; v1; v2; v3].
-Definition adderTree4_v0_v1_v2_v3 := unIdent (adderTree4 v0_v1_v2_v3).
 Example sum_v0_v1_v2_v3 :
-  Bv2N (unIdent (adderTree4 v0_v1_v2_v3)) = 30.
+  Bv2N (adderTree4 v0_v1_v2_v3) = 30.
 Proof. reflexivity. Qed.
 
 Local Open Scope nat_scope.
@@ -112,7 +111,7 @@ Definition adder_tree4_8_tb_inputs
       [9; 56; 2; 87];   [14; 72; 90; 11]; [64; 12; 92; 13];    [88; 24; 107; 200]]).
 
 Definition adder_tree4_8_tb_expected_outputs
-  := multistep (Comb adderTree4) adder_tree4_8_tb_inputs.
+  := simulate (Comb adderTree4) adder_tree4_8_tb_inputs.
 
 Definition adder_tree4_8_tb :=
   testBench "xadder_tree4_8_tb" adder_tree4_8Interface
@@ -132,21 +131,21 @@ Proof. reflexivity. Qed.
 Definition adder_tree32_8Interface := adder_tree_Interface "xadder_tree32_8" 32 8.
 
 Definition adder_tree32_8Netlist
-  := makeNetlist adder_tree32_8Interface (adderTree 4).
+  := makeNetlist adder_tree32_8Interface (adderTree 5).
 
 (* Create netlist and test-bench for a 64-input adder tree. *)
 
 Definition adder_tree64_8Interface := adder_tree_Interface "xadder_tree64_8" 64 8.
 
 Definition adder_tree64_8Netlist
-  := makeNetlist adder_tree64_8Interface (adderTree 5).
+  := makeNetlist adder_tree64_8Interface (adderTree 6).
 
 Definition adder_tree64_8_tb_inputs
   := map (fun i => Vector.map (N2Bv_sized 8) (Vector.map N.of_nat i))
      [vseq 0 64; vseq 64 64; vseq 128 64].
 
 Definition adder_tree64_8_tb_expected_outputs
-  := multistep (Comb (adderTree 5)) adder_tree64_8_tb_inputs.
+  := simulate (Comb (adderTree 6)) adder_tree64_8_tb_inputs.
 
 Definition adder_tree64_8_tb :=
   testBench "xadder_tree64_8_tb" adder_tree64_8Interface
@@ -159,7 +158,7 @@ Definition adder_tree64_8_tb :=
 Definition adder_tree64_128Interface := adder_tree_Interface "xadder_tree64_128" 64 128.
 
 Definition adder_tree64_128Netlist
-  := makeNetlist adder_tree64_128Interface (adderTree 5).
+  := makeNetlist adder_tree64_128Interface (adderTree 6).
 
 Definition adder_tree64_128_tb_inputs
   := map (fun i => Vector.map (N2Bv_sized 128) i)
@@ -167,7 +166,7 @@ Definition adder_tree64_128_tb_inputs
      [vseq 0 64; vseq 64 64; vseq 128 64]).
 
 Definition adder_tree64_128_tb_expected_outputs
-  := multistep (Comb (adderTree 5)) adder_tree64_128_tb_inputs.
+  := simulate (Comb (adderTree 6)) adder_tree64_128_tb_inputs.
 
 Definition adder_tree64_128_tb :=
   testBench "xadder_tree64_128_tb" adder_tree64_128Interface
@@ -180,7 +179,7 @@ Definition adder_tree64_128_tb :=
 Definition adder_tree128_256Interface := adder_tree_Interface "xadder_tree128_256" 128 256.
 
 Definition adder_tree128_256Netlist
-  := makeNetlist adder_tree128_256Interface (adderTree 6).
+  := makeNetlist adder_tree128_256Interface (adderTree 7).
 
 Definition adder_tree128_256_tb_inputs : list (Vector.t (Bvector 256) 128)
   := map (fun i => Vector.map (N2Bv_sized 256) i)
@@ -189,7 +188,7 @@ Definition adder_tree128_256_tb_inputs : list (Vector.t (Bvector 256) 128)
 
 Definition adder_tree128_256_tb_expected_outputs
            : list (Bvector 256)
-  := multistep (Comb (adderTree 6)) adder_tree128_256_tb_inputs.
+  := simulate (Comb (adderTree 7)) adder_tree128_256_tb_inputs.
 
 Definition adder_tree128_256_tb :=
   testBench "xadder_tree128_256_tb" adder_tree128_256Interface
