cava/Cava/Acorn/Acorn.v
@@ -14,11 +14,11 @@
 (* limitations under the License.                                           *)
 (****************************************************************************)
 
-Require Export Cava.Signal.
-Require Export Cava.Acorn.CavaClass.
-Require Export Cava.Acorn.CavaPrelude.
-Require Export Cava.Acorn.Circuit.
-Require Export Cava.Acorn.Combinational.
-Require Export Cava.Acorn.Combinators.
-Require Export Cava.Acorn.NetlistGeneration.
-Require Export Cava.Acorn.Multistep.
+Require Export Cava.Core.Signal.
+Require Export Cava.Core.CavaClass.
+Require Export Cava.Lib.CavaPrelude.
+Require Export Cava.Core.Circuit.
+Require Export Cava.Semantics.Combinational.
+Require Export Cava.Lib.Combinators.
+Require Export Cava.NetlistGeneration.NetlistGeneration.
+Require Export Cava.Semantics.Simulation.
