silveroak-opentitan/aes/Acorn/CipherEquivalence.v
@@ -23,28 +23,29 @@ Import VectorNotations.
 Import ListNotations.
 
 Require Import ExtLib.Structures.Monads.
-Open Scope monad_scope.
 
 Require Import coqutil.Tactics.Tactics.
-Require Import Cava.BitArithmetic.
-Require Import Cava.NatUtils.
-Require Import Cava.ListUtils.
-Require Import Cava.VectorUtils.
-Require Import Cava.Tactics.
+Require Import Cava.Util.BitArithmetic.
+Require Import Cava.Util.Nat.
+Require Import Cava.Util.List.
+Require Import Cava.Util.Vector.
+Require Import Cava.Util.Tactics.
 
 Require Import Cava.Acorn.Acorn.
-Require Import Cava.Acorn.Circuit.
-Require Import Cava.Acorn.Combinational.
-Require Import Cava.Acorn.CombinationalProperties.
-Require Import Cava.Acorn.Identity.
-Require Import Cava.Acorn.Multistep.
+Require Import Cava.Core.Circuit.
+Require Import Cava.Semantics.Combinational.
+Require Import Cava.Semantics.CombinationalProperties.
+Require Import Cava.Util.Identity.
+Require Import Cava.Semantics.Simulation.
 Require Import Cava.Lib.MultiplexersProperties.
 
 Require Import AesSpec.Cipher.
 Require Import AesSpec.CipherProperties.
 Require Import AcornAes.CipherCircuit.
 
-Existing Instance Combinational.CombinationalSemantics.
+Local Open Scope list_scope.
+Local Open Scope monad_scope.
+Existing Instance CombinationalSemantics.
 
 Local Notation byte := (Vector.t bool 8).
 Local Notation state := (Vector.t (Vector.t byte 4) 4) (only parsing).
@@ -82,16 +83,16 @@ Section WithSubroutines.
           (add_round_key_spec : state -> key -> state).
   Context
     (sub_bytes_correct : forall (is_decrypt : bool) (st : state),
-        unIdent (sub_bytes is_decrypt st)
+        sub_bytes is_decrypt st
         = if is_decrypt then inv_sub_bytes_spec st else sub_bytes_spec st)
     (shift_rows_correct : forall (is_decrypt : bool) (st : state),
-        unIdent (shift_rows is_decrypt st)
+        shift_rows is_decrypt st
         = if is_decrypt then inv_shift_rows_spec st else shift_rows_spec st)
     (mix_columns_correct : forall (is_decrypt : bool) (st : state),
-        unIdent (mix_columns is_decrypt st)
+        mix_columns is_decrypt st
         = if is_decrypt then inv_mix_columns_spec st else mix_columns_spec st)
     (add_round_key_correct :
-       forall k (st : state), unIdent (add_round_key k st) = add_round_key_spec st k).
+       forall k (st : state), add_round_key k st = add_round_key_spec st k).
 
   (* Formula for each round based on index *)
   Let round_spec (Nr : nat) (is_decrypt : bool) (k : key) (st : state) (i : nat) : state :=
@@ -132,13 +133,13 @@ Section WithSubroutines.
                      then if Nat.eqb i 0 then false
                           else if Nat.eqb i Nr then false else true
                      else false) ->
-    unIdent (cipher_round
-               (key:=Vec (Vec (Vec Bit 8) 4) 4)
-               (state:=Vec (Vec (Vec Bit 8) 4) 4)
-               (round_index:=Vec Bit 4)
-               sub_bytes shift_rows mix_columns add_round_key (mix_columns true)
-               is_decrypt k add_round_key_in_sel round_key_sel
-               (nat_to_bitvec_sized _ i) data)
+    cipher_round
+      (key:=Vec (Vec (Vec Bit 8) 4) 4)
+      (state:=Vec (Vec (Vec Bit 8) 4) 4)
+      (round_index:=Vec Bit 4)
+      sub_bytes shift_rows mix_columns add_round_key (mix_columns true)
+      is_decrypt k add_round_key_in_sel round_key_sel
+      (nat_to_bitvec_sized _ i) data
     = round_spec Nr is_decrypt k data i.
   Proof.
     cbv zeta; intros. subst_lets. subst. destruct_products.
@@ -155,14 +156,13 @@ Section WithSubroutines.
     1 < Nr < 2 ^ 4 -> i <= Nr ->
     num_regular_rounds = nat_to_bitvec_sized _ Nr ->
     is_first_round = (i =? 0)%nat ->
-    unIdent
-      (cipher_step
-         (key:=Vec (Vec (Vec Bit 8) 4) 4)
-         (state:=Vec (Vec (Vec Bit 8) 4) 4)
-         (round_index:=Vec Bit 4)
-         sub_bytes shift_rows mix_columns add_round_key (mix_columns true)
-         is_decrypt is_first_round num_regular_rounds
-         k (nat_to_bitvec_sized _ i) data)
+    cipher_step
+      (key:=Vec (Vec (Vec Bit 8) 4) 4)
+      (state:=Vec (Vec (Vec Bit 8) 4) 4)
+      (round_index:=Vec Bit 4)
+      sub_bytes shift_rows mix_columns add_round_key (mix_columns true)
+      is_decrypt is_first_round num_regular_rounds
+      k (nat_to_bitvec_sized _ i) data
     = round_spec Nr is_decrypt k data i.
   Proof.
     cbv zeta; intro Hall_keys; intros. subst.
@@ -244,14 +244,14 @@ Section WithSubroutines.
                   (state:=Vec (Vec (Vec Bit 8) 4) 4)
                   (round_index:=Vec Bit 4)
                   sub_bytes shift_rows mix_columns add_round_key (mix_columns true) in
-    multistep loop (combine cipher_input round_keys)
+    simulate loop (combine cipher_input round_keys)
     = cipher_trace_with_keys Nr is_decrypt init_state round_keys.
   Proof.
     cbv zeta; intros. subst cipher_input.
     cbv [make_cipher_signals] in *.
     destruct round_keys; cbn [length] in *; [ length_hammer | ].
     destruct init_key_ignored; cbn [length] in *; [ length_hammer | ].
-    cbv [multistep cipher_trace_with_keys].
+    cbv [simulate cipher_trace_with_keys].
     cbn [seq map combine].
     rewrite fold_left_accumulate_cons_full.
     cbn [tl].
@@ -377,7 +377,7 @@ Section WithSubroutines.
     cipher_input = make_cipher_signals Nr is_decrypt init_key_input
                                        (init_state :: init_state_ignored) ->
     (* precomputed keys match key expansion *)
-    multistep key_expand cipher_input = init_key :: middle_keys ++ [last_key] ->
+    simulate key_expand cipher_input = init_key :: middle_keys ++ [last_key] ->
     let cipher := cipher
                     (key:=Vec (Vec (Vec Bit 8) 4) 4)
                     (state:=Vec (Vec (Vec Bit 8) 4) 4)
@@ -385,7 +385,7 @@ Section WithSubroutines.
                     sub_bytes shift_rows mix_columns add_round_key (mix_columns true)
                     key_expand in
     forall d,
-      nth Nr (multistep cipher cipher_input) d
+      nth Nr (simulate cipher cipher_input) d
       = if is_decrypt
         then
           Cipher.equivalent_inverse_cipher
@@ -398,12 +398,12 @@ Section WithSubroutines.
             mix_columns_spec init_key last_key middle_keys init_state.
   Proof.
     cbv zeta; intros. subst cipher_input.
-    cbv [cipher]. autorewrite with push_multistep.
+    cbv [cipher]. autorewrite with push_simulate.
     rewrite !map_map.
-    rewrite !ListUtils.map_id_ext by reflexivity.
+    rewrite !List.map_id_ext by reflexivity.
     erewrite cipher_loop_equiv with (Nr:=Nr) (init_state_ignored:=init_state_ignored)
       by length_hammer.
-    match goal with Hkexp : multistep key_expand _ = _ |- _ =>
+    match goal with Hkexp : simulate key_expand _ = _ |- _ =>
                     cbv [combType Bvector.Bvector] in Hkexp |- *;
                       rewrite Hkexp; clear Hkexp end.
     cbv [cipher_trace_with_keys]. simplify.
