silveroak-opentitan/aes/Spec/CipherProperties.v
@@ -15,7 +15,7 @@
 (****************************************************************************)
 
 Require Import Coq.Lists.List.
-Require Import Cava.ListUtils.
+Require Import Cava.Util.List.
 Require Import AesSpec.Cipher.
 
 Section ChangeRepresentation.
