tests/AddWithDelay/ListProofs.v
@@ -25,11 +25,11 @@ Export MonadNotation.
 Require Import coqutil.Tactics.Tactics.
 
 Require Import Cava.Cava.
-Require Import Cava.ListUtils.
-Require Import Cava.Tactics.
+Require Import Cava.Util.List.
+Require Import Cava.Util.Tactics.
 Require Import Cava.Acorn.Acorn.
-Require Import Cava.Acorn.Identity.
-Require Import Cava.Acorn.CombinationalProperties.
+Require Import Cava.Util.Identity.
+Require Import Cava.Semantics.CombinationalProperties.
 Require Import Cava.Lib.UnsignedAdders.
 Import Circuit.Notations.
 
@@ -55,7 +55,7 @@ Definition addWithDelaySpecF
     end.
 
 Lemma addNCorrect n (a b : combType (Vec Bit n)) :
-  unIdent (addN (a, b)) = bvadd a b.
+  addN (a, b) = bvadd a b.
 Admitted.
 Hint Rewrite addNCorrect using solve [eauto] : simpl_ident.
 
@@ -88,11 +88,11 @@ Proof.
 Qed.
 
 Lemma addWithDelayCorrect (i : list (Bvector 8)) :
-  multistep addWithDelay i = map (fun t => addWithDelaySpecF (fun n => nth n i bvzero) t)
+  simulate addWithDelay i = map (fun t => addWithDelaySpecF (fun n => nth n i bvzero) t)
                                  (seq 0 (length i)).
 Proof.
   intros; cbv [addWithDelay].
-  eapply multistep_Loop_invariant
+  eapply simulate_Loop_invariant
     with (body:=(Comb addN >==> Delay >==> Comb fork2))
          (I := fun t st body_st acc =>
                  st = match t with
